unique_ids_loops.thy
@@ -6,6 +6,135 @@ begin
 
 text "We show that programs using the loop language are well formed with respect to unique identifiers."
 
+lemma invocations_cannot_guess_ids_io:
+  assumes proc_initial: "\<And>proc store localKnown cmd impl. 
+    procedure progr proc = ((store, localKnown, cmd), impl) \<Longrightarrow> 
+      impl = toImpl
+      \<and> localKnown = uniqueIds proc"
 
+shows "invocations_cannot_guess_ids progr"
+  unfolding invocations_cannot_guess_ids_def
+proof
+  fix i
+
+  have always_toImpl: "impl = toImpl"
+    if "initialState progr ~~ tr \<leadsto>* S"
+      and "currentProc S i \<triangleq> impl"
+    for tr S impl
+    using that
+  proof (induct rule: steps_induct)
+    case initial
+    then show ?case
+      by (simp add: initialState_def)
+  next
+    case (step S' tr a S'')
+    then show ?case 
+      by (auto simp add: step.simps proc_initial prog_initial steps_do_not_change_prog split: if_splits)
+  qed
+
+  have localKnownTi: "localKnown = trace_inputs tr i"
+    if "initialState progr ~~ tr \<leadsto>* S"
+      and "localState S i \<triangleq> (store, localKnown, cmd)"
+    for tr S store localKnown cmd
+    using that
+  proof (induct  arbitrary: store localKnown cmd rule: steps_induct)
+    case initial
+    then show ?case 
+      by (simp add: initialState_def)
+  next
+    case (step S' tr a S'')
+
+
+    show ?case
+    proof (cases "currentProc S' i \<triangleq> toImpl")
+      case False
+      hence "currentProc S' i = None"
+        using always_toImpl exists_optionI step.steps by blast
+
+      with step 
+      show "localKnown = trace_inputs (tr @ [a]) i"
+        using proc_initial 
+        by (auto simp add: step.simps proc_initial prog_initial steps_do_not_change_prog trace_inputs_append trace_inputs_cons trace_inputs_empty trace_inputs_if_no_op split: if_splits,
+            use proc_initial in \<open>blast+\<close>)
+    next
+      case True
+
+      from this 
+      obtain store1 localKnown1 cmd1
+        where ls: "localState S' i \<triangleq> (store1, localKnown1, cmd1)"
+        using wf_localState_currentProc_m
+        by (metis (no_types, hide_lams) exists_optionI option.distinct(1) prod_cases3 state_wellFormed_init step.steps wf_localState_currentProc)
+
+      have IH: "localKnown1 = trace_inputs tr i"
+        by (simp add: ls step.IH)
+
+      show "localKnown = trace_inputs (tr @ [a]) i"
+      proof (cases "fst a = i")
+        case False
+        with step
+        show ?thesis 
+          by (auto simp add: step.simps trace_inputs_append trace_inputs_cons trace_inputs_empty)
+      next
+        case True
+
+        from `S' ~~ a \<leadsto> S''`
+        have "S' ~~ (i, get_action a)  \<leadsto> S''"
+          using True by auto
+
+
+        from this                                           
+        have  "localKnown = localKnown1 \<union> action_inputs (get_action a)"
+          using ls[simplified IH] `currentProc S' i \<triangleq> toImpl` `localState S'' i \<triangleq> (store, localKnown, cmd)` IH
+          by (auto simp add: step.simps elim!: toImpl.elims split: if_splits prod.splits)
+
+        thus "localKnown = trace_inputs (tr @ [a]) i"
+          by (simp add: IH True trace_inputs_append trace_inputs_cons trace_inputs_empty)
+      qed
+    qed
+  qed
+
+
+  show "invocation_cannot_guess_ids {} i (initialState progr)"
+  proof (rule show_invocation_cannot_guess_ids)
+    fix x tr a S'
+    assume a0: "initialState progr ~~ tr @ [(i, a)] \<leadsto>* S'"
+      and a1: "x \<in> action_outputs a"
+      and a2: "x \<notin> {}"
+
+    from a0
+    obtain S where "initialState progr ~~ tr \<leadsto>* S" and "S ~~ (i, a) \<leadsto> S'"
+      using steps_appendBack by blast
+
+    show "x \<in> trace_inputs tr i"
+    proof (cases "localState S i")
+      case None
+      then show ?thesis 
+        using `S ~~ (i, a) \<leadsto> S'` `x \<in> action_outputs a`
+        by (auto simp add: step.simps)
+    next
+      case (Some ls)
+      from this
+      obtain store1 cmd1
+        where ls: "localState S i \<triangleq> (store1, trace_inputs tr i, cmd1)"
+        using \<open>initialState progr ~~ tr \<leadsto>* S\<close> localKnownTi 
+        by (metis prod_cases3)
+
+      hence "currentProc S i \<triangleq> toImpl"
+        by (smt \<open>initialState progr ~~ tr \<leadsto>* S\<close> always_toImpl not_Some_eq state_wellFormed_init wf_localState_currentProc wf_localState_currentProc_m)
+
+
+
+
+      from `S ~~ (i, a) \<leadsto> S'`
+        and `localState S i \<triangleq> (store1, trace_inputs tr i, cmd1)`
+        and `currentProc S i \<triangleq> toImpl`
+        and `x \<in> action_outputs a`
+      show ?thesis 
+        by (cases cmd1, auto simp add: step.simps split: prod.splits if_splits)
+    qed
+  qed
+qed
+
+   
 
 end
